CoqBB5/BB5/Prelims.v
@@ -3,9 +3,7 @@ Require Import ZArith.
 Require Import FSets.FMapPositive.
 
 From CoqBB5 Require Import BB5_Statement.
-From CoqBB5 Require Import Custom_Tactics.
-
-Definition BB5_minus_one:N := 47176869.
+From CoqBB5 Require Import Tactics.
 
 Definition Dir_rev(d:Dir) :=
 match d with
@@ -107,23 +105,8 @@ Proof.
   rewrite PositiveMap.gempty in H. cg.
 Qed.
 
-Definition St_list:= St0::St1::St2::St3::St4::nil.
-Definition Σ_list:= Σ0::Σ1::nil.
+
 Definition Dir_list := Dpos::Dneg::nil.
-
-Lemma St_list_spec:
-  forall s, In s St_list.
-Proof.
-  intro s.
-  destruct s; cbn; tauto.
-Qed.
-
-Lemma Σ_list_spec:
-  forall s, In s Σ_list.
-Proof.
-  intro s.
-  destruct s; cbn; tauto.
-Qed.
 
 Lemma Dir_list_spec:
   forall s, In s Dir_list.
@@ -132,34 +115,10 @@ Proof.
   destruct s; cbn; tauto.
 Qed.
 
-Definition forallb_St f :=
-  forallb f St_list.
-
-Definition forallb_Σ f :=
-  forallb f Σ_list.
 
 Definition forallb_Dir f :=
   forallb f Dir_list.
 
-Lemma forallb_St_spec f:
-  forallb_St f = true <-> forall s, f s = true.
-Proof.
-  unfold forallb_St.
-  rewrite forallb_forall.
-  split; intros.
-  - apply H,St_list_spec.
-  - apply H.
-Qed.
-
-Lemma forallb_Σ_spec f:
-  forallb_Σ f = true <-> forall s, f s = true.
-Proof.
-  unfold forallb_Σ.
-  rewrite forallb_forall.
-  split; intros.
-  - apply H,Σ_list_spec.
-  - apply H.
-Qed.
 
 Lemma forallb_Dir_spec f:
   forallb_Dir f = true <-> forall s, f s = true.
@@ -185,21 +144,3 @@ Qed.
 
 Ltac Dir_eq_dec s1 s2 :=
   eq_dec Dir_eqb_spec Dir_eqb s1 s2.
-
-Inductive DeciderIdentifier : Type :=
-| DECIDER_NIL (* Definition HaltDecider_nil:HaltDecider := fun _ => Result_Unknown. *)
-| LOOP1_params_130 (* decider2 *)
-| NGRAM_CPS_IMPL2_params_1_1_100 (* decider3 *)
-| NGRAM_CPS_IMPL2_params_2_2_200 (* decider4 *)
-| NGRAM_CPS_IMPL2_params_3_3_400 (* decider5 *)
-| NGRAM_CPS_IMPL1_params_2_2_2_1600 (* decider6 *)
-| NGRAM_CPS_IMPL1_params_2_3_3_1600 (* decider7 *)
-| LOOP1_params_4100 (* decider8 *)
-| NGRAM_CPS_IMPL1_params_4_2_2_600 (* decider9 *)
-| NGRAM_CPS_IMPL1_params_4_3_3_1600 (* decider10 *)
-| NGRAM_CPS_IMPL1_params_6_2_2_3200 (* decider11 *)
-| NGRAM_CPS_IMPL1_params_6_3_3_3200 (* decider12 *)
-| NGRAM_CPS_IMPL1_params_8_2_2_1600 (* decider13 *)
-| NGRAM_CPS_IMPL1_params_8_3_3_1600 (* decider14 *)
-| TABLE_BASED (* table_based_decider *)
-| NORMAL_FORM_TABLE_BASED. (* NF_decider table_based_decider, meaning 1RB normalisation is applied before lookeup *)
