CoqBB5/BB5/TNF_Roots/TNF_Root_4/TNF_Root_4_3_leaf.v
@@ -1,4 +1,4 @@
-(* TNF Root 1RB---_1RA---_------_------_------ *)
+(* TNF Root 1RB---_0RA---_------_------_------ *)
 
 Require Import ZArith.
 Require Import List.
@@ -6,7 +6,7 @@ Require Import Lia.
 
 From CoqBB5 Require Import Tactics.
 From CoqBB5 Require Import Prelims.
-From CoqBB5 Require Import Encodings.
+From CoqBB5 Require Import BB5_Encodings.
 From CoqBB5 Require Import TNF.
 From CoqBB5 Require Import TM.
 From CoqBB5 Require Import BB5_Statement.
@@ -16,21 +16,22 @@ From CoqBB5 Require Import BB5_Deciders_Pipeline.
 
 Definition q_1_manual := (SearchQueue_upds root4_q decider_all 0).
 
-Definition q_4_trivial_2 := nth 3 (fst q_1_manual) root.
-Definition q_4_trivial_2' : SearchQueue := q_suc (SearchQueue_init q_4_trivial_2).
+Definition q_4_trivial_1 := nth 2 (fst q_1_manual) root.
 
-Lemma q_4_trivial_2'_nil :
-  q_4_trivial_2' = (nil, nil).
+Definition q_4_trivial_1' : SearchQueue := q_suc (SearchQueue_init q_4_trivial_1).
+
+Lemma q_4_trivial_1'_nil :
+  q_4_trivial_1' = (nil, nil).
 Proof.
   reflexivity.
 Qed.
 
-Lemma q_4_trivial_2'_WF:
-  SearchQueue_WF (N.to_nat BB5_minus_one) q_4_trivial_2' q_4_trivial_2.
+Lemma q_4_trivial_1'_WF:
+  SearchQueue_WF (N.to_nat BB5_minus_one) q_4_trivial_1' q_4_trivial_1.
 Proof.
-  unfold q_4_trivial_2'.
-  change ((q_suc (SearchQueue_init q_4_trivial_2))) with
-    (Nat.iter 1 q_suc (SearchQueue_init q_4_trivial_2)).
+  unfold q_4_trivial_1'.
+  change ((q_suc (SearchQueue_init q_4_trivial_1))) with
+    (Nat.iter 1 q_suc (SearchQueue_init q_4_trivial_1)).
   apply q_200_WF_gen.
   red. repeat split.
   1: cbn; cg.
@@ -48,12 +49,12 @@ Proof.
   congruence.
 Qed.
 
-Lemma q_4_trivial_2_HTUB:
-  TNF_Node_HTUB (N.to_nat BB5_minus_one) q_4_trivial_2.
+Lemma q_4_trivial_1_HTUB:
+  TNF_Node_HTUB (N.to_nat BB5_minus_one) q_4_trivial_1.
 Proof.
-  epose proof q_4_trivial_2'_WF.
+  epose proof q_4_trivial_1'_WF.
   unfold SearchQueue_WF in H.
-  rewrite q_4_trivial_2'_nil in H.
+  rewrite q_4_trivial_1'_nil in H.
   apply H.
   cbn.
   intros.
