CoqBB5/BB5/BB5_Make_TM.v
@@ -1,0 +1,132 @@
+Require Import ZArith.
+Require Import Lia.
+Require Import List.
+
+From CoqBB5 Require Import BB5_Statement.
+From CoqBB5 Require Import TM.
+From CoqBB5 Require Import List_Routines.
+From CoqBB5 Require Import Tactics.
+From CoqBB5 Require Import Prelims.
+From CoqBB5 Require Import BB5_Encodings.
+
+
+Definition AL0 := Some {| nxt:=St0; dir:=Dneg; out:=Σ0 |}.
+Definition AL1 := Some {| nxt:=St0; dir:=Dneg; out:=Σ1 |}.
+Definition AR0 := Some {| nxt:=St0; dir:=Dpos; out:=Σ0 |}.
+Definition AR1 := Some {| nxt:=St0; dir:=Dpos; out:=Σ1 |}.
+
+Definition BL0 := Some {| nxt:=St1; dir:=Dneg; out:=Σ0 |}.
+Definition BL1 := Some {| nxt:=St1; dir:=Dneg; out:=Σ1 |}.
+Definition BR0 := Some {| nxt:=St1; dir:=Dpos; out:=Σ0 |}.
+Definition BR1 := Some {| nxt:=St1; dir:=Dpos; out:=Σ1 |}.
+
+Definition CL0 := Some {| nxt:=St2; dir:=Dneg; out:=Σ0 |}.
+Definition CL1 := Some {| nxt:=St2; dir:=Dneg; out:=Σ1 |}.
+Definition CR0 := Some {| nxt:=St2; dir:=Dpos; out:=Σ0 |}.
+Definition CR1 := Some {| nxt:=St2; dir:=Dpos; out:=Σ1 |}.
+
+Definition DL0 := Some {| nxt:=St3; dir:=Dneg; out:=Σ0 |}.
+Definition DL1 := Some {| nxt:=St3; dir:=Dneg; out:=Σ1 |}.
+Definition DR0 := Some {| nxt:=St3; dir:=Dpos; out:=Σ0 |}.
+Definition DR1 := Some {| nxt:=St3; dir:=Dpos; out:=Σ1 |}.
+
+Definition EL0 := Some {| nxt:=St4; dir:=Dneg; out:=Σ0 |}.
+Definition EL1 := Some {| nxt:=St4; dir:=Dneg; out:=Σ1 |}.
+Definition ER0 := Some {| nxt:=St4; dir:=Dpos; out:=Σ0 |}.
+Definition ER1 := Some {| nxt:=St4; dir:=Dpos; out:=Σ1 |}.
+
+Definition HL0:option (Trans Σ) := None.
+Definition HL1:option (Trans Σ) := None.
+Definition HR0:option (Trans Σ) := None.
+Definition HR1:option (Trans Σ) := None.
+
+Definition makeTM:
+(option (Trans Σ))->(option (Trans Σ))->
+(option (Trans Σ))->(option (Trans Σ))->
+(option (Trans Σ))->(option (Trans Σ))->
+(option (Trans Σ))->(option (Trans Σ))->
+(option (Trans Σ))->(option (Trans Σ))->
+(TM Σ) :=
+fun A0 A1 B0 B1 C0 C1 D0 D1 E0 E1 s i =>
+match s,i with
+| St0,Σ0 => A0
+| St0,Σ1 => A1
+| St1,Σ0 => B0
+| St1,Σ1 => B1
+| St2,Σ0 => C0
+| St2,Σ1 => C1
+| St3,Σ0 => D0
+| St3,Σ1 => D1
+| St4,Σ0 => E0
+| St4,Σ1 => E1
+end.
+
+Definition Trans_list:=
+{| nxt:=St0; dir:=Dneg; out:=Σ0 |}::
+{| nxt:=St0; dir:=Dneg; out:=Σ1 |}::
+{| nxt:=St0; dir:=Dpos; out:=Σ0 |}::
+{| nxt:=St0; dir:=Dpos; out:=Σ1 |}::
+{| nxt:=St1; dir:=Dneg; out:=Σ0 |}::
+{| nxt:=St1; dir:=Dneg; out:=Σ1 |}::
+{| nxt:=St1; dir:=Dpos; out:=Σ0 |}::
+{| nxt:=St1; dir:=Dpos; out:=Σ1 |}::
+{| nxt:=St2; dir:=Dneg; out:=Σ0 |}::
+{| nxt:=St2; dir:=Dneg; out:=Σ1 |}::
+{| nxt:=St2; dir:=Dpos; out:=Σ0 |}::
+{| nxt:=St2; dir:=Dpos; out:=Σ1 |}::
+{| nxt:=St3; dir:=Dneg; out:=Σ0 |}::
+{| nxt:=St3; dir:=Dneg; out:=Σ1 |}::
+{| nxt:=St3; dir:=Dpos; out:=Σ0 |}::
+{| nxt:=St3; dir:=Dpos; out:=Σ1 |}::
+{| nxt:=St4; dir:=Dneg; out:=Σ0 |}::
+{| nxt:=St4; dir:=Dneg; out:=Σ1 |}::
+{| nxt:=St4; dir:=Dpos; out:=Σ0 |}::
+{| nxt:=St4; dir:=Dpos; out:=Σ1 |}::
+nil.
+
+Lemma Trans_list_spec:
+  forall tr, In tr Trans_list.
+Proof.
+  intro.
+  destruct tr as [s d o].
+  cbn.
+  destruct s,d,o; tauto.
+Qed.
+
+Definition Σ_history_enc(x:Σ_history):positive:=
+  let (x0,x1):=x in
+  match x0 with
+  | Σ0 => (listStΣ_enc x1)~0
+  | Σ1 => (listStΣ_enc x1)~1
+  end.
+
+Lemma Σ_history_enc_inj: is_inj Σ_history_enc.
+Proof.
+  intros x1 x2 H.
+  destruct x1 as [a1 b1].
+  destruct x2 as [a2 b2].
+  cbn in H.
+  destruct a1,a2; invst H; f_equal; apply listStΣ_enc_inj,H1.
+Qed.
+
+Definition TM_enc(tm:TM Σ):positive :=
+  match TM_to_N tm with
+  | N0 => xH
+  | Npos v => Pos.succ v
+  end.
+
+Definition TM_simplify tm :=
+  makeTM
+  (tm St0 Σ0) (tm St0 Σ1)
+  (tm St1 Σ0) (tm St1 Σ1)
+  (tm St2 Σ0) (tm St2 Σ1)
+  (tm St3 Σ0) (tm St3 Σ1)
+  (tm St4 Σ0) (tm St4 Σ1).
+
+Lemma TM_simplify_spec tm:
+  TM_simplify tm = tm.
+Proof.
+  unfold TM_simplify,makeTM.
+  fext. fext.
+  destruct x,x0; reflexivity.
+Qed.
