CoqBB5/BB5/Deciders/Decider_Halt.v
@@ -3,10 +3,12 @@ Require Import ZArith.
 
 From CoqBB5 Require Import TM.
 From CoqBB5 Require Import BB5_Statement.
-From CoqBB5 Require Import Custom_Tactics.
+From CoqBB5 Require Import Tactics.
 From CoqBB5 Require Import TNF.
 From CoqBB5 Require Import List_Tape.
 From CoqBB5 Require Import Prelims.
+From CoqBB5 Require Import BB5_Encodings.
+From CoqBB5 Require Import Deciders_Common.
 
 Set Warnings "-abstract-large-number".
 
@@ -109,24 +111,3 @@ Proof.
     + cbn in H.
       specialize (IHn (Pos.pred_N p) H). lia.
 Qed.
-
-Definition halt_decider_max := halt_decider 47176870.
-Lemma halt_decider_max_spec: HaltDecider_WF (N.to_nat BB5_minus_one) halt_decider_max.
-Proof.
-  eapply halt_decider_WF.
-  unfold BB5_minus_one.
-  replace (S (N.to_nat 47176869)) with (N.to_nat 47176870) by lia.
-  replace (Init.Nat.of_num_uint
-    (Number.UIntDecimal
-       (Decimal.D4
-          (Decimal.D7
-             (Decimal.D1
-                (Decimal.D7 (Decimal.D6 (Decimal.D8 (Decimal.D7 (Decimal.D0 Decimal.Nil))))))))))
-  with (N.to_nat 47176870).
-  1: apply Nat.le_refl.
-  symmetry.
-  apply nat_eqb_N_spec.
-  vm_compute.
-  reflexivity.
-Qed.
-
