CoqBB5/BB5/Deciders/Decider_Loop.v
@@ -4,11 +4,12 @@ Require Import ZArith.
 
 From CoqBB5 Require Import TM.
 From CoqBB5 Require Import BB5_Statement.
-From CoqBB5 Require Import Custom_Tactics.
+From CoqBB5 Require Import Tactics.
 From CoqBB5 Require Import TNF.
 From CoqBB5 Require Import List_Tape.
 From CoqBB5 Require Import Prelims.
-From CoqBB5 Require Import Encodings.
+From CoqBB5 Require Import BB5_Encodings.
+From CoqBB5 Require Import Deciders_Common.
 
 (* Begin: Loop decider implementation *)
 
