CoqBB5/BB5/Deciders/Verifier_FAR.v
@@ -5,14 +5,16 @@ Require Import Lia.
 Require Import List.
 Require Import ZArith.
 
-From CoqBB5 Require Import Custom_Tactics.
-From CoqBB5 Require Import Encodings.
+From CoqBB5 Require Import Tactics.
+From CoqBB5 Require Import BB5_Encodings.
 From CoqBB5 Require Import BB5_Statement.
 From CoqBB5 Require Import Prelims.
 From CoqBB5 Require Import List_Tape.
 From CoqBB5 Require Import Decider_RepWL.
 From CoqBB5 Require Import TM.
 From CoqBB5 Require Import TNF.
+From CoqBB5 Require Import Deciders_Common.
+
 
 Section DFA_NFA_verifier.
 
