CoqBB5/BB5/Deciders_Hardcoded_Parameters/Decider_Loop_Hardcoded_Parameters.v
@@ -1,7 +1,8 @@
 Require Import List.
 
 From CoqBB5 Require Import TM.
-From CoqBB5 Require Import BB5_Decider_Pipeline.
+From CoqBB5 Require Import BB5_Make_TM.
+From CoqBB5 Require Import BB5_Deciders_Hardcoded.
 
 Definition tm_Lp1 :=
 (makeTM BR1 HR1 CL1 EL0 DR1 BL0 DR0 AR1 CL0 AR0,Lp1)::
