CoqBB5/BB5/List_Tape.v
@@ -3,11 +3,12 @@ Require Import List.
 Require Import Lia.
 
 From CoqBB5 Require Import Prelims.
-From CoqBB5 Require Import Encodings.
+From CoqBB5 Require Import BB5_Encodings.
 From CoqBB5 Require Import TM.
+From CoqBB5 Require Import BB5_Make_TM.
 From CoqBB5 Require Import BB5_Statement.
-From CoqBB5 Require Import Custom_Tactics.
-From CoqBB5 Require Import Custom_List_Routines.
+From CoqBB5 Require Import Tactics.
+From CoqBB5 Require Import List_Routines.
 From CoqBB5 Require Import Decider_NGramCPS.
 From CoqBB5 Require Import TNF.
 
